Walkup.thy
@@ -10,74 +10,19 @@ text \<open>Special case for triangular identity - either merge two cycles or sp
 definition skip_edge where
 "skip_edge z h x \<equiv> if z = x then z else
                   (if (edge h z) = z then edge h x else
-                  (if (face h (edge h x)) = z then edge h z else
+                  (if x = node h z then edge h z else
                   (if edge h x = z then edge h (node h z) else edge h x)))"
-
-text \<open>This definition follows Stahl's 1983 paper, with P and Q swapped\<close>
-definition skip_edge_alt where
-"skip_edge_alt z h x \<equiv>
- skip z (edge h * cycle_perm (cycle_of_list [z, node h (face h z), node h z])) x"
-
-lemma (in hypermap) skip_edge_altdef:
-  assumes "node H z \<noteq> z"
-  shows "skip_edge z H = skip_edge_alt z H" (is "?L = ?R")
-proof
-  fix x consider
-    (id) "x = z"
-    | (edge_z) "x \<noteq> z \<and> (edge H z) = z" 
-    | (face_edge)"x \<noteq> z \<and> (edge H z) \<noteq> z \<and> face H (edge H x) = z" 
-    | (edge_x) "x \<noteq> z \<and> (edge H z) \<noteq> z \<and> face H (edge H x) \<noteq> z \<and> edge H x = z" 
-    | (no_match) "x \<noteq> z \<and> (edge H z) \<noteq> z \<and> face H (edge H x) \<noteq> z \<and> edge H x \<noteq> z"
-    by auto
-  then show "?L x = ?R x"
-proof cases
-  case id then show ?thesis
-    by (simp add: skip_edge_def skip_edge_alt_def)
-next
-  case edge_z
-  then have "?L x = edge H x" by (metis skip_edge_def)
-  also have "?R x = edge H x"
-    by (metis skip_z_eq_fz cycle_of_list_not_distinct cycle_perm_id distinct_length_2_or_more
-        edge_z mult.right_neutral nodeK skip_edge_alt_def)
-  finally show ?thesis by simp
-next
-  case face_edge then show ?thesis
-    by (smt (verit, ccfv_threshold) apply_inj_eq_iff apply_perm_sequence apply_perm_swap(2)
- cycle_of_list_not_distinct cycle_perm_cycle_of_list_doubleton cycle_perm_id skip_edge_alt_def
- cycle_perm_of_list_Cons_Cons distinct_length_2_or_more edgeK mult.right_neutral skip_def skip_edge_def)
-next
-  case edge_x
-  then have "skip_edge z H x = edge H (node H z)"
-    by (metis skip_edge_def)
-  moreover {
-    from edge_x have "edge H x = z" by simp
-    then have "x = node H (face H z)"
-      using nodeK by force
-    then have "(cycle_perm (cycle_of_list [z, node H (face H z), node H z])) x = node H z"
-      using assms edge_x by force
-    hence "?R x = edge H (node H z)"
-      by (metis \<open>x = (node H) \<langle>$\<rangle> (face H) \<langle>$\<rangle> z\<close> apply_inj_eq_iff 
-          apply_perm_sequence edge_x skip_invariant skip_edge_alt_def)
-  }
-  ultimately show ?thesis by simp
-next
-  case no_match 
-  then have "?L x = edge H x" by (metis skip_edge_def)
-  also 
-  { have "cycle_perm (cycle_of_list [z, node H (face H z), node H z]) x = x"
-      by (smt (verit, ccfv_SIG) apply_cycle_of_list apply_perm_cycle apply_perm_swap(3)
-          cycle_lookup_hd cycle_perm_cycle_of_list_doubleton cycle_perm_same_iff
-          distinct_length_2_or_more hypermap.edgeK hypermap.faceK hypermap_axioms insert_iff
-          list.simps(15) no_match perm_eq_iff set_cycle_code)
-    then have "?R x = edge H x" unfolding skip_edge_alt_def
-      by (simp add: apply_perm_times no_match skip_def)
-  }
-  finally show ?thesis by simp
-qed
-qed
 
 lemma skip_edge_id [simp]: "skip_edge z h z = z"
   unfolding skip_edge_def by simp
+
+lemma skip_edge_noteq_z: "x \<noteq> z \<Longrightarrow> skip_edge z H x \<noteq> z"
+  by (metis apply_inj_eq_iff skip_edge_def)
+
+lemma (in hypermap) skip_edge_base:
+  assumes "x \<noteq> z" "x \<noteq> node H (face H z)" "x \<noteq> node H z"
+  shows "edge H x = skip_edge z H x"
+  by (metis assms nodeK skip_edge_def)
 
 context hypermap 
 begin
@@ -93,9 +38,11 @@ proof
     show "\<And>x. x \<in> (A - {z}) \<Longrightarrow> skip_edge z H x \<in> (A - {z})"
       by (smt (z3) Diff_iff \<open>A = darts H\<close> apply_inj_eq_iff empty_iff faceK
           perm_edge perm_face insert_iff permutes_in_image skip_edge_def)
-    show "\<And>x. x \<notin> (A - {z}) \<Longrightarrow> skip_edge z H x = x"
-      by (smt (z3) Diff_empty Diff_insert0 Permutations.permutes_not_in \<open>A = darts H\<close>
-          perm_edge perm_face insert_Diff insert_iff skip_edge_def)
+    have "set_perm (node H) \<subseteq> darts H"
+      by (simp add: perm_node perm_on.intro perm_on.set_perm_subset)
+    then show "\<And>x. x \<notin> (A - {z}) \<Longrightarrow> skip_edge z H x = x"
+      by (smt (z3) Diff_iff Permutations.permutes_not_in \<open>A = darts H\<close> apply_perm_image
+          empty_iff imageI insert_iff perm_edge skip_edge_def)
   qed
 qed
 
@@ -108,7 +55,8 @@ proof
     then have disj: "x \<notin> darts H \<or> x = z" by simp
     have "x = z \<Longrightarrow> skip_edge z H x = x" by simp
     also have "x \<notin> darts H \<Longrightarrow> skip_edge z H x = x"
-      by (metis Permutations.permutes_not_in perm_edge perm_face skip_edge_def)
+      by (metis (no_types, lifting) Permutations.permutes_not_in
+          faceK perm_edge perm_face skip_edge_def)
     ultimately show "skip_edge z H x = x"
       using disj by linarith
     qed
@@ -121,10 +69,7 @@ qed
 lemma skip_edgeK: "skip_edge z H (skip z (node H) (skip z (face H) x)) = x"
   by (smt (z3) edgeK faceK nodeK skip_def skip_edge_def)
 
-lemma skip_edge_noteq_z: "x \<noteq> z \<Longrightarrow> skip_edge z H x \<noteq> z"
-  by (metis apply_inj_eq_iff skip_edge_Perm skip_edge_id)
-
-lemma (in hypermap) glink_skip_edge: "z\<rightarrow>\<^bsub>glink H\<^esub>z \<Longrightarrow> skip_edge z H = skip z (edge H)"
+lemma (in hypermap) glink_fp_skip_edge: "z\<rightarrow>\<^bsub>glink H\<^esub>z \<Longrightarrow> skip_edge z H = skip z (edge H)"
 proof
   fix x assume *: "z\<rightarrow>\<^bsub>glink H\<^esub>z"
   then have z_eq: "z = edge H z \<or> z = node H z \<or> z = face H z"
@@ -133,8 +78,8 @@ proof
     by (simp add: skip_def skip_edge_def)
   also have "z = node H z \<Longrightarrow> skip_edge z H x = skip z (edge H) x"
     unfolding skip_edge_def skip_def using * nodeK by fastforce
-  moreover have "z = face H z \<Longrightarrow> skip_edge z H x = skip z (edge H) x"
-    unfolding skip_edge_def skip_def using * faceK by auto
+  moreover have "z = face H z \<Longrightarrow> skip_edge z H x = skip z (edge H) x" 
+    by (smt (z3) skip_edge_def skip_def * faceK edgeK nodeK)
   ultimately show "skip_edge z H x = skip z (edge H) x"
     using z_eq by blast
 qed
@@ -149,9 +94,28 @@ definition walkupE :: "'a pre_hypermap \<Rightarrow> 'a \<Rightarrow> 'a pre_hyp
    node = skip_perm z (node h),
    face = skip_perm z (face h)\<rparr>"
 
+theorem (in hypermap) hypermap_walkupE:
+  shows "hypermap (walkupE H z)"
+proof
+  define H' where "H' \<equiv> walkupE H z"
+  have "finite (darts H)" by (rule finite_darts)
+  also have "darts H' = darts H - {z}"
+    by (simp add: H'_def walkupE_def)
+  ultimately show "finite (darts H')" by auto
+  show "edge H' permutes darts H'"
+    by (simp add: H'_def finite_darts hypermap_axioms permutes_perm skip_edge_permutes walkupE_def)
+  show "node H' permutes darts H'"
+    by (simp add: H'_def walkupE_def apply_skip_perm perm_node skip_permutes)
+  show "face H' permutes darts H'"
+    by (simp add: H'_def walkupE_def apply_skip_perm perm_face skip_permutes)
+  fix x show "(edge H') \<langle>$\<rangle> (node H') \<langle>$\<rangle> (face H') \<langle>$\<rangle> x = x"
+    by (simp add: H'_def skip_edgeK apply_skip_perm skip_edge_Perm walkupE_def)
+qed
+
 locale walkup = hypermap +
   fixes z
   assumes z_dart: "z \<in> darts H"
+
 begin
   definition "H' \<equiv> walkupE H z"
 
@@ -163,24 +127,18 @@ lemma walkup_node: "node H' = skip_perm z (node H)"
 
 lemma walkup_face: "face H' = skip_perm z (face H)"
   by (simp add: H'_def walkupE_def)
-end
 
+lemma walkup_darts_subset: "darts H' \<subseteq> darts H"
+  unfolding H'_def walkupE_def by simp
+end
+(*
 locale not_degenerate_walkup = walkup +
-  fixes u v
   assumes z_not_glink: "\<not>z\<rightarrow>\<^bsub>glink H\<^esub>z"
-      and dart_u: "u \<in> darts H'"
-      and dart_v: "v \<in> darts H'"
 begin
 
-lemma u_noteq_z: "u \<noteq> z"
-  by (metis dart_u DiffE H'_def insert_iff pre_hypermap.select_convs(1) walkupE_def)
-
-lemma v_noteq_z: "v \<noteq> z"
-  by (metis dart_v DiffE H'_def insert_iff pre_hypermap.select_convs(1) walkupE_def)
-
 lemma skip_edge_edge: "skip_edge z H (node H (face H z)) = (edge H (node H z))"
-  unfolding skip_edge_def
-  by (metis Gr_eq cedge_def cface_def edgeK glink_def pair_union_arcs_disj z_dart z_not_glink)
+  by (smt (z3) Gr_eq arc_in_union cedge_def darts_permF edgeK faceK glink_def permF_def permF_glink
+      pre_hypermap.select_convs(2) skip_edge_def z_dart z_not_glink)
 
 lemma skip_edge_node: "skip_edge z H (node H z) = (edge H z)"
   unfolding skip_edge_def
@@ -189,33 +147,17 @@ lemma skip_edge_node: "skip_edge z H (node H z) = (edge H z)"
 
 lemma skip_edge_invariant:
   fixes x
-  assumes "x \<noteq> z" "face H (edge H x) \<noteq> z" "edge H x \<noteq> z"
+  assumes "x \<noteq> z" "node H z \<noteq> x" "edge H x \<noteq> z"
   shows "skip_edge z H x = edge H x"
   unfolding skip_edge_def using assms by auto
 
 lemma walkup_darts_subset: "darts H' \<subseteq> darts H"
   unfolding H'_def walkupE_def by simp
 end
+*)
 
 context walkup 
 begin
-theorem hypermap_walkupE:
-  shows "hypermap H'"
-proof
-  have "finite (darts H)" by (rule finite_darts)
-  also have "(darts H') = (darts H) - {z}"
-    by (simp add: H'_def walkupE_def)
-  ultimately show "finite (darts H')" by auto
-  show "edge H' permutes darts (H')"
-    by (simp add: H'_def finite_darts hypermap_axioms permutes_perm skip_edge_permutes walkupE_def)
-  show "(node (H')) permutes darts (H')"
-    by (simp add: H'_def walkupE_def apply_skip_perm perm_node skip_permutes)
-  show "(face (H')) permutes darts (H')"
-    by (simp add: H'_def walkupE_def apply_skip_perm perm_face skip_permutes)
-  fix x show "(edge (H')) \<langle>$\<rangle> (node (H')) \<langle>$\<rangle> (face (H')) \<langle>$\<rangle> x = x"
-    by (simp add: H'_def skip_edgeK apply_skip_perm skip_edge_Perm walkupE_def)
-qed
-
 lemma card_darts_walkup: "card (darts H') = card (darts H) - 1"
   by (simp add: H'_def finite_darts walkupE_def z_dart)
 
@@ -229,23 +171,11 @@ text \<open>(From fourcolour.walkup.v)
 
 definition "cross_edge \<equiv> z\<rightarrow>\<^sup>*\<^bsub>cedge H\<^esub>node H z"
 
-lemma cross_edge_path_edge:
-  "cross_edge \<longleftrightarrow> edge H z\<rightarrow>\<^sup>*\<^bsub>cedge H\<^esub>node H z" (is "?L = ?R")
-proof
-  assume ?L show ?R
-  proof (rule wf_digraph.reachable_trans)
-    show "wf_digraph (cedge H)"
-      by (simp add: wf_cedge wf_digraph_wp_iff)
-    then show "(edge H) \<langle>$\<rangle> z \<rightarrow>\<^sup>*\<^bsub>with_proj (cedge H)\<^esub> z"
-      by (metis Gr_eq cedge_connect_sym cedge_def wf_digraph.reach_sym_arc z_dart)
-    show "z \<rightarrow>\<^sup>*\<^bsub>with_proj (cedge H)\<^esub> (node H) \<langle>$\<rangle> z"
-      using \<open>cross_edge\<close> unfolding cross_edge_def by simp
-  qed
-next
-  assume ?R then show ?L
-    by (metis Gr_eq cedge_def cross_edge_def wf_cedge wf_digraph.adj_reachable_trans 
-        wf_digraph_wp_iff z_dart)
-qed
+(*
+lemma cross_edge_path_edge: "cross_edge \<longleftrightarrow> edge H z\<rightarrow>\<^sup>*\<^bsub>cedge H\<^esub>node H z"
+  by (metis (no_types, hide_lams) Gr_eq cedge_connect_sym cedge_def cross_edge_def wf_cedge
+      wf_digraph.connect_sym_def wf_digraph.reachable_adjI wf_digraph.reachable_trans 
+      wf_digraph_wp_iff z_dart)*)
 
 interpretation clink: fin_digraph "clink H"
   by (simp add: finite_clink)
@@ -254,8 +184,8 @@ definition z_comp where
 "z_comp \<equiv> (clink H') \<restriction> (clink.scc_of z - {z})"
 
 lemma wf_z_comp: "wf_digraph z_comp"
-   by (simp add: fin_digraph.axioms(1) hypermap.finite_clink hypermap_walkupE 
-        wf_digraph.wellformed_induce_subgraph z_comp_def)
+  by (simp add: H'_def hypermap.wf_clink hypermap_walkupE 
+      wf_digraph.wellformed_induce_subgraph wf_digraph_wp_iff z_comp_def)
 
 interpretation z_comp: fin_digraph z_comp
 proof intro_locales
@@ -272,8 +202,8 @@ proof intro_locales
     then have "arcs z_comp \<subseteq> arcs (clink H')"
       by (simp add: z_comp_def)
     then have "finite (arcs z_comp)"
-      by (meson fin_digraph.finite_arcs finite_subset hypermap.finite_clink hypermap_walkupE)
-  }
+    by (metis H'_def fin_digraph.finite_arcs hypermap.finite_clink hypermap_walkupE rev_finite_subset)
+    }
   ultimately show "fin_digraph_axioms z_comp"
     using fin_digraph_axioms.intro by blast
 qed
@@ -283,7 +213,7 @@ definition z_barb where
 
 lemma z_barb_z: "z_barb = (edge H z = z \<and> node H z = z \<and> face H z = z)"
 proof
-  assume *: "z_barb"
+  assume "z_barb"
   then show "edge H z = z \<and> node H z = z \<and> face H z = z"
     by (smt (verit) DiffD2 apply_inj_eq_iff clink.in_sccs_verts_conv_reachable
         clink.scc_of_in_sccs_verts clinkN clink_connect_sym fst_conv hypermap.clinkF hypermap_axioms
@@ -317,80 +247,31 @@ next
     using clink.wf_digraph_axioms clinkF pre_digraph.scc_of_def wf_digraph.adj_in_verts(1)
       z_barb_def z_dart by fastforce
 qed
-                                                    
-lemma z_barb_comp: "z_barb = (pre_digraph.sccs z_comp = {})"
-proof
-  assume z_barb
-  then have "verts z_comp = {}"
-    unfolding z_barb_def z_comp_def by simp
-  moreover have "arcs z_comp = {}"
-    by (metis wf_z_comp calculation ex_in_conv wf_digraph.wellformed(2))
-  ultimately show "pre_digraph.sccs z_comp = {}"
-    by (metis antisym_conv bot.extremum equals0I pre_digraph.in_sccsE
-        pre_digraph.induced_subgraph_altdef strongly_connected_def subgraph_def)
-next
-  assume "pre_digraph.sccs z_comp = {}"
-  then have "verts z_comp = {}"
-    by (metis empty_iff equals0I wf_digraph.in_verts_sccsD_sccs 
-        wf_digraph.scc_of_in_sccs_verts wf_z_comp) 
-  then have "clink.scc_of z - {z} = {}"
-    using z_comp_def by force 
-  then have "clink.scc_of z = {z}"
-    by (metis clink.adj_in_verts(2) clink.in_scc_of_self
-        clinkN insert_Diff walkup.z_dart walkup_axioms)
-  then show z_barb
-    unfolding H'_def z_comp_def z_barb_def by blast
-qed
 
-
-definition "disconnected \<equiv> card (pre_digraph.sccs z_comp) > 1"
-
-lemma disconnected_not_glink: "disconnected \<Longrightarrow> \<not> z\<rightarrow>\<^bsub>glink H\<^esub>z"
-proof
-  assume *: disconnected "z\<rightarrow>\<^bsub>glink H\<^esub>z"
-  then have "\<not>z_barb"
-    using disconnected_def z_barb_comp by force
-  have "strongly_connected z_comp"
-  proof
-    show "verts z_comp \<noteq> {}"
-      using \<open>\<not> z_barb\<close> z_barb_comp z_comp.sccs_conv_sccs_verts z_comp.sccs_verts_conv_scc_of
-      by force
-    show "u \<in> verts z_comp \<Longrightarrow> v \<in> verts z_comp \<Longrightarrow> u \<rightarrow>\<^sup>*\<^bsub>z_comp\<^esub> v" for u v
-      sorry
-  qed
-  then have "card (pre_digraph.sccs z_comp) = 1"
-    using wf_digraph.card_sccs_connected wf_z_comp by blast
-  then show False
-    using *(1) disconnected_def by linarith
-qed
-
-lemma disconnected_cross_edge: "disconnected \<Longrightarrow> cross_edge"
-  sorry
-
-corollary not_cross_connected: "\<not> cross_edge \<Longrightarrow> \<not> disconnected"
-  using disconnected_cross_edge by auto
-
-lemma (in not_degenerate_walkup) clink_at_G': "u \<rightarrow>\<^bsub>clink H\<^esub>v \<Longrightarrow> u\<rightarrow>\<^bsub>clink H'\<^esub>v"
+lemma clink_at_H':
+  assumes "u \<in> darts H'" "v \<in> darts H'"
+  shows "u \<rightarrow>\<^bsub>clink H\<^esub>v \<Longrightarrow> u\<rightarrow>\<^bsub>clink H'\<^esub>v"
 proof -
   assume "u \<rightarrow>\<^bsub>clink H\<^esub>v"
   then have "(v\<rightarrow>\<^bsub>cnode H\<^esub> u \<or> u \<rightarrow>\<^bsub>cface H\<^esub> v)" (is "?N \<or> ?F")
     by (metis clink_def converse_iff pair_pre_digraph.simps(2) pair_union_arcs_disj
         reverse_def with_proj_simps(3))
   also have "v\<rightarrow>\<^bsub>cnode H\<^esub> u \<Longrightarrow> v\<rightarrow>\<^bsub>cnode H'\<^esub> u"
-    by (metis Gr_eq H'_def apply_skip_perm cnode_def dart_v pre_hypermap.select_convs(3)
-        skip_def u_noteq_z v_noteq_z walkupE_def)
+    by (metis DiffD2 Gr_eq H'_def apply_skip_perm assms cnode_def insertCI 
+        pre_hypermap.select_convs(1) skip_invariant walkupE_def walkup_node)
   moreover have "u \<rightarrow>\<^bsub>cface H\<^esub> v \<Longrightarrow> u \<rightarrow>\<^bsub>cface H'\<^esub> v"
-    by (metis Gr_eq H'_def apply_skip_perm cface_def dart_u pre_hypermap.select_convs(4)
-        skip_def u_noteq_z v_noteq_z walkupE_def)
+    by (metis DiffD2 Gr_eq H'_def apply_skip_perm assms(1) assms(2) cface_def 
+        pre_hypermap.select_convs(1) singleton_iff skip_invariant walkupE_def walkup_face)
   ultimately show ?thesis
-    by (meson dart_u dart_v hypermap.clinkP hypermap_walkupE)
+    by (metis H'_def hypermap.clinkP hypermap_walkupE)
 qed
 
-lemma (in not_degenerate_walkup) clink_at_H:
+lemma clink_at_H:
+  assumes "u \<in> darts H'" "v \<in> darts H'"
   shows "u \<rightarrow>\<^sup>*\<^bsub>clink H'\<^esub>v \<Longrightarrow> u\<rightarrow>\<^sup>*\<^bsub>clink H\<^esub>v"
 proof -
   interpret clink': wf_digraph "clink H'"
-    using hypermap.wf_clink hypermap_walkupE wf_digraph_wp_iff by blast
+    by (simp add: H'_def hypermap.wf_clink hypermap_walkupE wf_digraph_wp_iff)
   interpret clink: wf_digraph "clink H"
     by (simp add: wf_clink wf_digraph_wp_iff)
   assume "u \<rightarrow>\<^sup>*\<^bsub>clink H'\<^esub>v"
@@ -405,9 +286,10 @@ proof -
     case (Cons w)
     then have "w \<in> darts H'"
       unfolding clink_def cface_def cnode_def by (simp add: reverse_def)
+    then have "w \<in> darts H"
+      using walkup_darts_subset by force
     then have "w \<in> verts (clink H)"
-      unfolding clink_def cface_def cnode_def reverse_def 
-      using walkup_darts_subset by auto
+      using verts_clink by blast
     then have "clink.awalk w [] w"
       by (simp add: clink.awalk_Nil_iff)
     then show ?case by blast
@@ -488,246 +370,232 @@ proof -
     using clink.reachable_awalk by blast
 qed
 
+lemma z_comp_clink: "x \<in> verts z_comp \<longleftrightarrow> (x\<rightarrow>\<^sup>*\<^bsub>clink H\<^esub>z \<and> x \<noteq> z)"
+proof safe
+  show "x \<in> verts z_comp \<Longrightarrow> x \<rightarrow>\<^sup>*\<^bsub>clink H\<^esub> z"
+    by (simp add: pre_digraph.scc_of_def z_comp_def)
+  show "z \<in> verts z_comp \<Longrightarrow> x = z \<Longrightarrow> False"
+    by (simp add: z_comp_def)
+  then have "x \<in> clink.scc_of z" if "x\<rightarrow>\<^sup>*\<^bsub>clink H\<^esub>z"
+    using clink.connect_sym_def clink.scc_of_def clink_connect_sym that by blast
+  then show "x \<in> verts z_comp" if "x \<noteq> z" "x\<rightarrow>\<^sup>*\<^bsub>clink H\<^esub>z"
+    by (simp add: that z_comp_def)
+qed
+
+lemma z_barb_comp: "z_barb = (pre_digraph.sccs z_comp = {})"
+proof
+  assume z_barb
+  then have "verts z_comp = {}"
+    unfolding z_barb_def z_comp_def by simp
+  moreover have "arcs z_comp = {}"
+    by (metis wf_z_comp calculation ex_in_conv wf_digraph.wellformed(2))
+  ultimately show "pre_digraph.sccs z_comp = {}"
+    by (metis antisym_conv bot.extremum equals0I pre_digraph.in_sccsE
+        pre_digraph.induced_subgraph_altdef strongly_connected_def subgraph_def)
+next
+  assume "pre_digraph.sccs z_comp = {}"
+  then have "verts z_comp = {}"
+    by (metis empty_iff equals0I wf_digraph.in_verts_sccsD_sccs 
+        wf_digraph.scc_of_in_sccs_verts wf_z_comp) 
+  then have "clink.scc_of z - {z} = {}"
+    using z_comp_def by force 
+  then have "clink.scc_of z = {z}"
+    by (metis clink.adj_in_verts(2) clink.in_scc_of_self
+        clinkN insert_Diff walkup.z_dart walkup_axioms)
+  then show z_barb
+    unfolding H'_def z_comp_def z_barb_def by blast
+qed
+
+lemma not_cross_edge_Walkup:
+  assumes "\<not> cross_edge" "edge H z \<in> darts H'"
+  shows "edge H z\<rightarrow>\<^sup>*\<^bsub>cedge H'\<^esub>node H (face H z)"
+proof -
+  have "z \<noteq> edge H z"
+    by (metis DiffD2 H'_def assms(2) insert_iff pre_hypermap.select_convs(1) walkupE_def)
+  then obtain p0 where p0_def: "vpath p0 (cedge H) \<and> hd p0 = edge H z \<and> last p0 = z"
+    by (metis Gr_eq cedge_connect_sym cedge_def wf_cedge wf_digraph.connect_sym_def
+        wf_digraph.reachable_adjI wf_digraph.reachable_vpath_conv wf_digraph_wp_iff z_dart)
+  then obtain p where p_def: "p0 = (p @ [z])"
+    by (smt (verit, ccfv_threshold) \<open>z \<noteq> (edge H) \<langle>$\<rangle> z\<close> last.simps last_appendR list.sel(1) 
+        neq_Nil_conv rev_exhaust vpathE vwalk_def)
+  then have "hd p = edge H z"
+    by (metis \<open>z \<noteq> (edge H) \<langle>$\<rangle> z\<close> hd_append list.sel(1) p0_def p_def)
+  then have vpath_p: "vpath p (cedge H)"
+    by (metis \<open>z \<noteq> (edge H) \<langle>$\<rangle> z\<close> hd_append list.sel(1) p0_def p_def vpath_sublist(1))
+  then have cedge_p: "x \<in> set p \<Longrightarrow> x\<rightarrow>\<^sup>*\<^bsub>cedge H\<^esub>z" for x
+  proof -
+    assume "x \<in> set p"
+    then obtain h q where "p = h @ (x#q)"
+      by (meson split_list)
+    then have "vpath (x#q) (cedge H)"
+      using vpath_p vpath_sublist(2) by auto
+    also have "last p\<rightarrow>\<^bsub>cedge H\<^esub> z"
+      by (metis \<open>p = h @ x # q\<close> p_def p0_def append_is_Nil_conv insert_subset list.distinct(1)
+          set_vwalk_arcs_snoc vpathE vwalk_def)
+    then have "vpath (x#q@[z]) (cedge H)"
+      using \<open>p = h @ x # q\<close> p0_def p_def vpath_sublist(2) by auto
+    then show ?thesis
+      by (metis append_is_Nil_conv last.simps last_snoc list.distinct(1) list.sel(1) wf_cedge
+          wf_digraph.reachable_vpath_conv wf_digraph_wp_iff)
+  qed
+  then have "z \<notin> set p"
+    using p_def p0_def vpath_def by auto
+  have "edge H (last p) = z"
+    by (metis p_def vpath_p p0_def Gr_eq cedge_def insert_subset set_vwalk_arcs_snoc vpathE vwalkE)
+  then have "last p = (node H (face H z))"
+    by (metis nodeK)
+  also have "vpath p (cedge H')"
+  proof (auto simp: vpath_def intro!: vwalkI)
+    show x_vert: "x \<in> set p \<Longrightarrow> x \<in> pverts (cedge H')" for x
+      by (metis Gr_verts H'_def \<open>z \<notin> set p\<close> cedge_def insert_Diff insert_iff
+          pre_hypermap.select_convs(1) vpathE vpath_p vwalk_verts_in_verts walkupE_def
+          with_proj_simps(1) z_dart)
+    show "p = [] \<Longrightarrow> False" "distinct p"
+      using vpath_p by blast+
+    fix a b assume *: "(a,b) \<in> set (vwalk_arcs p)"
+    then have "(a,b) \<in> parcs (cedge H)"
+      by (metis in_mono vpathE vpath_p vwalkE with_proj_simps(3))
+    then have "edge H a = b"
+      by (simp add: cedge_def)
+    also have "a \<noteq> node H (face H z)"
+      by (metis * \<open>z \<notin> set p\<close> calculation edgeK in_set_vwalk_arcsE)
+    moreover have "a \<noteq> z"
+      by (metis * \<open>z \<notin> set p\<close> in_set_vwalk_arcsE)
+    moreover have "a \<noteq> node H z"
+      by (metis assms(1) cedge_p "*" cedge_connect_sym cross_edge_def in_set_vwalk_arcsE wf_cedge
+          wf_digraph.connect_sym_def wf_digraph_wp_iff)
+    ultimately have "edge H' a = b"
+      using skip_edge_Perm skip_edge_base walkup_edge by force
+    then show "(a,b) \<in> parcs (cedge H')"
+      by (metis Gr_eq Gr_verts * \<open>\<And>x. x \<in> set p \<Longrightarrow> x \<in> pverts (cedge H')\<close> cedge_def 
+          in_set_vwalk_arcsE with_proj_simps(1) with_proj_simps(3))
+  qed
+  ultimately show ?thesis
+    by (metis H'_def \<open>hd p = (edge H) \<langle>$\<rangle> z\<close> hypermap.wf_cedge hypermap_walkupE
+        wf_digraph.reachable_vpath_conv wf_digraph_wp_iff)
+qed
+
+
+definition "disconnected \<equiv> card (pre_digraph.sccs z_comp) > 1"
+
+lemma disconnected_cross_edge: "disconnected \<Longrightarrow> \<not> z\<rightarrow>\<^bsub>glink H\<^esub>z \<and> cross_edge"
+proof -
+  assume *: "disconnected"
+  {
+    assume "\<not> (\<not> z\<rightarrow>\<^bsub>glink H\<^esub>z \<and> cross_edge)"
+    then obtain x where "x\<rightarrow>\<^bsub>clink H\<^esub>z \<and> x \<noteq> z"
+      by (metis "*" bot.extremum_strict bot_nat_def card.empty clinkN disconnected_def 
+          hypermap.clinkF hypermap.faceK hypermap_axioms perm_face permutes_in_image
+          walkup.z_barb_comp walkup.z_barb_z walkup.z_dart walkup_axioms)
+    then have "x \<in> darts H'"
+      by (metis H'_def fin_digraph.axioms(1) finite_clink insert_Diff insert_iff 
+          pre_hypermap.select_convs(1) verts_clink walkupE_def wf_digraph.adj_in_verts(1) z_dart)
+    then have "v \<in> darts H' \<Longrightarrow> v \<in> verts z_comp = (v\<rightarrow>\<^sup>*\<^bsub>clink H'\<^esub> x)" for v
+      sorry
+    then have "card (pre_digraph.sccs z_comp) = 1"
+      sorry
+  }
+  then show ?thesis
+    using "*" disconnected_def by force
+qed
+
+corollary not_cross_connected: "\<not> cross_edge \<Longrightarrow> \<not> disconnected"
+  using disconnected_cross_edge by auto
+
 definition "skip_edge_domain \<equiv> {x. x\<rightarrow>\<^sup>*\<^bsub>cedge H\<^esub>z \<or> x\<rightarrow>\<^sup>*\<^bsub>cedge H\<^esub>node H z}"
 
 lemma eCedom: "x \<in> skip_edge_domain \<Longrightarrow> edge H x \<in> skip_edge_domain"
   apply (auto simp: skip_edge_domain_def)
   by (metis Gr_eq Gr_verts cedge_connect_sym cedge_def pre_digraph.converse_reachable_cases wf_cedge 
       wf_digraph.reach_sym_arc wf_digraph_wp_iff)+
-end
-
-context not_degenerate_walkup
-begin
 
 lemma same_cskip_edge:
-  assumes "u \<notin> skip_edge_domain"
+  assumes "u \<notin> skip_edge_domain" "u \<in> darts H'"
   shows "u\<rightarrow>\<^sup>*\<^bsub>cedge H\<^esub>v \<longleftrightarrow> u\<rightarrow>\<^sup>*\<^bsub>cedge H'\<^esub>v"
-proof -
-  have "(((\<langle>$\<rangle>) (edge H')^^m) u = ((\<langle>$\<rangle>) (edge H)^^m) u)" for m
+proof (cases "z\<rightarrow>\<^bsub>glink H\<^esub>z")
+  case True
+  then show ?thesis sorry
+next
+  case False
+  have *: "((\<langle>$\<rangle>) (edge H')^^m) u = ((\<langle>$\<rangle>) (edge H)^^m) u" for m
   proof (induct m)
     case 0 then show ?case by simp
   next
     case (Suc m)
     then show ?case
-      by (smt (verit, best) assms cedge_def dart_u funpow_simp_l in_mono mem_Collect_eq nodeK
-          not_degenerate_walkup.skip_edge_invariant not_degenerate_walkup_axioms perm_edge
-          perm_on.intro perm_on.reach_iff_funpow_perm skip_edge_Perm skip_edge_domain_def
-          walkup_darts_subset walkup_edge)
+      by (smt (verit, best) assms cedge_def funpow_simp_l in_mono mem_Collect_eq perm_edge
+          perm_on.intro perm_on.reach_iff_funpow_perm skip_edge_Perm skip_edge_def
+          skip_edge_domain_def walkup_darts_subset walkup_edge)
   qed
   then show ?thesis
-    by (smt (verit, del_insts) cedge_def dart_u hypermap.perm_edge hypermap_walkupE
-        not_degenerate_walkup.walkup_darts_subset not_degenerate_walkup_axioms perm_edge
-        perm_on.intro perm_on.reach_iff_funpow_perm subsetD)
+    by (smt (verit) H'_def assms(2) cedge_def hypermap.perm_edge hypermap_walkupE *
+     walkup_darts_subset perm_edge perm_on.intro perm_on.reach_iff_funpow_perm subsetD)
 qed
 
-lemma sub_cskip_edge: "\<not> cross_edge \<Longrightarrow> u\<rightarrow>\<^sup>*\<^bsub>cedge H\<^esub>v \<Longrightarrow> u\<rightarrow>\<^sup>*\<^bsub>cedge H'\<^esub>v"
+lemma sub_cskip_edge:
+  assumes "\<not> cross_edge" "u \<in> darts H'" "v \<in> darts H'"
+  shows "u\<rightarrow>\<^sup>*\<^bsub>cedge H\<^esub>v \<Longrightarrow> u\<rightarrow>\<^sup>*\<^bsub>cedge H'\<^esub>v"
   sorry
 
 lemma cskip_edge_merge: 
-  assumes "\<not> cross_edge" "u \<in> skip_edge_domain"
+  assumes "\<not> cross_edge" "u \<in> skip_edge_domain" "u \<in> darts H'" "v \<in> darts H'"
   shows "u\<rightarrow>\<^sup>*\<^bsub>cedge H'\<^esub>v \<longleftrightarrow> v \<in> skip_edge_domain"
 proof
   show "v \<in> skip_edge_domain" if "u\<rightarrow>\<^sup>*\<^bsub>cedge H'\<^esub>v"
-    by (smt (verit, ccfv_SIG) hypermap.wf_cedge assms(2) that dart_u dart_v wf_digraph_wp_iff 
-    hypermap_walkupE mem_Collect_eq not_degenerate_walkup.intro not_degenerate_walkup.same_cskip_edge 
-    not_degenerate_walkup_axioms.intro skip_edge_domain_def walkup_axioms wf_cedge z_not_glink
-    wf_digraph.reachable_trans wf_digraph.connect_sym_def hypermap.cedge_connect_sym)
+    sorry
   assume *: "v \<in> skip_edge_domain"
   have "node H (face H z) \<noteq> z"
-      by (metis Gr_eq assms(1) cedge_def cross_edge_path_edge edgeK skip_edge_node skip_edge_noteq_z 
-          wf_cedge wf_digraph.reachable_adjI wf_digraph_wp_iff z_dart)
+    sorry
   then have "edge H z \<noteq> z"
-      by (metis nodeK)
+    by (metis nodeK)
   then show "u\<rightarrow>\<^sup>*\<^bsub>cedge H'\<^esub>v"
-      using * assms apply_inj_eq_iff apply_skip_perm perm.apply_perm_inverse pre_hypermap.select_convs(2) skip_edge_Perm skip_id u_noteq_z walkupE_def sorry
+    using assms sorry
 qed
+
 
 lemma fcard_skip_edge:
   defines "Sez \<equiv> if z \<rightarrow>\<^bsub>glink H\<^esub> z 
                  then (if edge H z = z then 2 else 1) 
                  else (if cross_edge then 0 else 2)"
   shows "count_cycles_on (darts H') (edge H') + Sez = count_cycles_on (darts H) (edge H) + 1"
-  apply (auto simp: Sez_def)
-  using with_proj_simps(3) z_not_glink apply blast
-  apply (metis Gr_eq arc_in_union cedge_def glink_def with_proj_simps(3) z_dart)
-  apply (metis Gr_eq cedge_def cross_edge_def skip_edge_node skip_edge_noteq_z wf_cedge
-      wf_digraph.reachable_adjI wf_digraph_wp_iff z_dart)
-  using with_proj_simps(3) z_not_glink apply blast
-  defer
-  using with_proj_simps(3) z_not_glink apply blast
-  sorry
-
-end
-subsection \<open>Degenerate walkup\<close>
-text \<open>Degenerate case for walkup where one of the permutations is an identity on z\<close>
-
-locale degenerate_walkup = walkup +
-  assumes z_glink: "z\<rightarrow>\<^bsub>glink H\<^esub> z"
-begin
-
-lemma degenerate_euler:
-  shows "euler_lhs H - euler_lhs H' = euler_rhs H - euler_rhs H'"
-proof (cases "edge H z = z \<and> node H z = z \<and> face H z = z")
-interpret face_perm_on: finite_perm_on "face H" "darts H"
-  by (rule finite_perm_on_face)
-interpret node_perm_on: finite_perm_on "node H" "darts H"
-  by (rule finite_perm_on_node)
-interpret edge_perm_on: finite_perm_on "edge H" "darts H"
-  by (rule finite_perm_on_edge)
+proof (cases "z\<rightarrow>\<^bsub>glink H\<^esub>z")
   case True
-  have "euler_rhs H' = euler_rhs H - 3"
-  proof -
-    have "count_cycles_on (darts H) (node H) = count_cycles_on (darts H') (node H') + 1"
-        by (metis True H'_def node_perm_on.cycle_count_skip_singleton finite_darts
-            pre_hypermap.select_convs(1) pre_hypermap.select_convs(3) walkupE_def z_dart)
-    also have "count_cycles_on (darts H) (face H) = count_cycles_on (darts H') (face H') + 1"
-        by (metis True H'_def face_perm_on.cycle_count_skip_singleton finite_darts
-            pre_hypermap.select_convs(1) pre_hypermap.select_convs(4) walkupE_def z_dart)
-    moreover have "count_cycles_on (darts H) (edge H) = count_cycles_on (darts H') (edge H') + 1"
-      by (metis True apply_skip_perm H'_def finite_darts glink_skip_edge perm.apply_perm_inverse
-          perm_edge perm_on.cycle_count_skip_singleton perm_on.intro pre_hypermap.select_convs(1)
-          pre_hypermap.select_convs(2) walkupE_def z_glink z_dart)
-    ultimately show ?thesis
-      by (simp add: euler_rhs_def)
-  qed
-  also have "euler_lhs H' = euler_lhs H - 3"
-  proof -
-    have "card (darts H') = card (darts H) - (1::int)" (is "?cdh' = ?cdh - 1")
-      using card_darts_walkup int_ops(6) node_perm_on.finite_S z_dart by auto
-    also have "int (card (pre_digraph.sccs (glink H'))) = int (card (pre_digraph.sccs (glink H))) - 1"
-      (is "?scch' = ?scch - 1")
-      sorry
-    then have "?scch' * (2::int) + ?cdh' = ?scch * (2::int) + ?cdh - (3::int)"
-      using calculation by fastforce
-    then show ?thesis
-      unfolding euler_lhs_def by presburger
-  qed
-  ultimately show ?thesis
-    by (metis diff_diff_cancel euler_lhs_ge_3 euler_rhs_ge_3 insert_absorb insert_not_empty z_dart)
+  then show ?thesis
+    apply (case_tac "edge H z = z")
+    apply (auto simp add: Sez_def)
+    by (smt (z3) H'_def Suc_eq_plus1 add.right_neutral True apply_perm_inject apply_skip_perm 
+        finite_darts hypermap.glink_fp_skip_edge hypermap.skip_edge_Perm hypermap_axioms perm_edge
+        perm_on.cycle_count_skip perm_on.intro pre_hypermap.select_convs(1) walkupE_def 
+        walkup_edge z_dart)+
 next
   case False
+  then have neq_z: "edge H z \<noteq> z \<and> node H z \<noteq> z \<and> face H z \<noteq> z \<and> node H (face H z) \<noteq> z"
+    by (metis Gr_eq arc_clink cedge_def clinkP edgeK glink_def pair_union_arcs_disj z_dart)
+  interpret H': hypermap "H'"
+    by (simp add: H'_def hypermap_walkupE)
+  have eCG: "x\<rightarrow>\<^sup>*\<^bsub>cedge H\<^esub>y \<Longrightarrow> y\<rightarrow>\<^sup>*\<^bsub>cedge H\<^esub>x" for x y
+    using cedge_connect_sym wf_cedge wf_digraph.connect_sym_def wf_digraph_wp_iff by blast
+  have eCG': "x\<rightarrow>\<^sup>*\<^bsub>cedge H'\<^esub>y \<Longrightarrow> y\<rightarrow>\<^sup>*\<^bsub>cedge H'\<^esub>x" for x y
+    using H'.cedge_connect_sym H'.wf_cedge wf_digraph.connect_sym_def wf_digraph_wp_iff by blast
   then show ?thesis sorry
 qed
-end
-
-subsection \<open>Not degenerate walkup\<close>
-context not_degenerate_walkup begin
-
-lemma walkup_node_cycle_count:
-  shows "count_cycles_on (darts H) (node H) = count_cycles_on (darts H') (node H')"
-proof -
-  interpret perm_on "(node H)" "(darts H)"
-    using perm_node perm_on.intro by blast
-  have "count_cycles_on (darts H) (node H) =
-        count_cycles_on (darts H - {z}) (skip_perm z (node H))"
-    apply (rule cycle_count_skip)
-      apply (simp_all add: z_dart finite_darts)
-      apply (metis z_not_glink Gr_eq arc_in_union cedge_def glink_def
-            skip_edge_id skip_edge_node z_dart)
-    done
-  then show ?thesis
-    by (simp add: H'_def walkupE_def)
-qed
-
-lemma walkup_face_cycle_count:
-  shows "count_cycles_on (darts H) (face H) = count_cycles_on (darts H') (face H')"
-proof -
-  interpret perm_on "(face H)" "(darts H)"
-    using perm_face perm_on.intro by blast
-  have "count_cycles_on (darts H) (face H) =
-        count_cycles_on (darts H - {z}) (skip_perm z (face H))"
-    apply (rule cycle_count_skip)
-      apply (simp_all add: z_dart finite_darts)
-      apply (metis Gr_eq arc_in_union cedge_def edgeK glink_def
-            skip_edge_edge skip_edge_node z_dart z_not_glink)
-    done
-  then show ?thesis
-    by (simp add: H'_def walkupE_def)
-qed
-
-text \<open>cross_edge does not hold, so the edge cycles are merged and edge z is in the same edge cycle
-      as node z\<close>
-
-lemma not_cross_edge_Walkup:
-  assumes "\<not> cross_edge"
-  shows "edge H z\<rightarrow>\<^sup>*\<^bsub>cedge H'\<^esub>node H (face H z)"
-  unfolding H'_def 
-  sorry
-
-lemma merge_walkup_path:
-  assumes "\<not> cross_edge"
-  shows "edge H z\<rightarrow>\<^sup>*\<^bsub>cedge H'\<^esub>node H z"
-  by (metis Gr_eq Gr_verts H'_def assms cedge_def hypermap.cedge_connect_sym hypermap.perm_edge
-      hypermap.wf_cedge hypermap_walkupE not_cross_edge_Walkup permutes_in_image reachable_in_vertsE
-      skip_edge_Perm skip_edge_node walkup_edge wf_digraph.reach_sym_arc wf_digraph_wp_iff)
-
-lemma merge_walkup_edge_cycles:
-  assumes  "\<not> cross_edge"
-  shows "count_cycles_on (darts H) (edge H) = count_cycles_on (darts H') (edge H') + 1"
- sorry
-
-lemma not_cross_edge_euler_lhs:
-  assumes "\<not> cross_edge"
-  shows "euler_rhs H = euler_rhs H' + 1"
-proof -
-  have "count_cycles_on (darts H) (face H) = count_cycles_on (darts H') (face H')"
-    by (simp add: assms walkup_face_cycle_count)
-  also have "count_cycles_on (darts H) (node H) = count_cycles_on (darts H') (node H')"
-    by (simp add: assms walkup_node_cycle_count)
-  moreover have "count_cycles_on (darts H) (edge H) = count_cycles_on (darts H') (edge H') + 1"
-    by (simp add: assms merge_walkup_edge_cycles)
-  ultimately show ?thesis
-    unfolding euler_rhs_def by simp
-qed
-
-lemma cross_edge_euler_rhs:
-  assumes "cross_edge"
-  shows "euler_rhs H = euler_rhs H' + 3"
-proof -
-  have "count_cycles_on (darts H) (face H) = count_cycles_on (darts H') (face H')"
-    by (simp add: assms walkup_face_cycle_count)
-  also have "count_cycles_on (darts H) (node H) = count_cycles_on (darts H') (node H')"
-    by (simp add: assms walkup_node_cycle_count)
-  moreover have "count_cycles_on (darts H) (edge H) = count_cycles_on (darts H') (edge H') + 3"
-    oops
-
-text \<open>cross_edge does not hold, so the edge cycle is split\<close>
-lemma (in not_degenerate_walkup) cross_edge_walkup:
-  assumes "cross_edge"
-  shows "\<not>edge H z\<rightarrow>\<^sup>*\<^bsub>cedge (walkupE H z)\<^esub>node H (face H z)"
-   using assms Gr_eq apply_inj_eq_iff apply_skip_perm arc_in_union cedge_def cface_def cnode_def
-      glink_def perm.apply_perm_inverse perm_eq_iff pre_hypermap.select_convs(2) skip_edge_Perm 
-      skip_id walkupE_def with_proj_simps(3) sorry
-end
 
 section \<open>Jordan and Euler\<close>
-context walkup
-begin
 
 definition "n_comp_z disc \<equiv> if z\<rightarrow>\<^bsub>glink H\<^esub>z
                               then (if z_barb then 2 else 1)
                               else (if disc then 0 else 1)"
 
-lemma euler_lhs_walkupE: "n_comp_z disconnected * 2 + euler_lhs H' = euler_lhs H + 1"
-  apply (auto simp: n_comp_z_def)
-  using disconnected_not_glink with_proj_simps(3) apply blast
-  apply (simp add: disconnected_def walkup.z_barb_comp walkup_axioms)
-  defer
-  apply (metis Gr_eq arc_in_union cedge_def glink_def with_proj_simps(3) z_barb_z z_dart)
-  using disconnected_not_glink apply auto
+lemma n_comp_glink_Walkup: "n_comp_z disconnected + card (pre_digraph.sccs (glink H'))
+                          = card (pre_digraph.sccs (glink H)) + 1"
   sorry
 
-lemma euler_rhs_walkupE: "n_comp_z disconnected * 2 + euler_rhs H' = euler_rhs H + 1"
-  apply (auto simp: n_comp_z_def)
-  using disconnected_not_glink with_proj_simps(3) apply blast
-  apply (simp add: disconnected_def walkup.z_barb_comp walkup_axioms)
-  defer
-  apply (metis Gr_eq arc_in_union cedge_def glink_def with_proj_simps(3) z_barb_z z_dart)
-  using disconnected_not_glink with_proj_simps(3) apply blast
-  sorry
+lemma euler_lhs_walkupE: "n_comp_z disconnected * 2 + euler_lhs H' = euler_lhs H + 1"
+  apply (simp add: euler_lhs_def)
+  by (metis One_nat_def Suc_pred add_2_eq_Suc add_Suc_right card_darts_walkup card_gt_0_iff
+      empty_iff finite_darts left_add_mult_distrib mult_2_right n_comp_glink_Walkup nat_1_add_1 z_dart)
 
 lemma genus_walkupE_eq: "z\<rightarrow>\<^bsub>glink H\<^esub>z \<or> \<not> cross_edge \<Longrightarrow> genus H' = genus H"
-  apply auto
   sorry
 
 lemma le_genus_walkupE: "genus H' \<le> genus H"
@@ -736,49 +604,347 @@ proof (cases "z\<rightarrow>\<^bsub>glink H\<^esub>z \<or> \<not> cross_edge")
   then show ?thesis using genus_walkupE_eq by force
 next
   case False
-  then have "\<not>z\<rightarrow>\<^bsub>glink H\<^esub>z \<and> cross_edge" by auto
-  then have "disconnected" sorry
+  have "count_cycles_on (darts H') (edge H') = count_cycles_on (darts H) (edge H) + 1"
+    using fcard_skip_edge False by presburger
+  moreover have "count_cycles_on (darts H') (node H') = count_cycles_on (darts H) (node H)"
+    by (smt (z3) False H'_def add.right_neutral arc_clink clinkP finite_darts glink_def 
+        pair_union_arcs_disj perm_node perm_on.cycle_count_skip perm_on.intro 
+        pre_hypermap.select_convs(1) pre_hypermap.select_convs(3) walkupE_def z_dart)
+  moreover have "count_cycles_on (darts H') (face H') = count_cycles_on (darts H) (face H)"
+    by (smt (z3) False H'_def add.right_neutral arc_clink clinkP finite_darts glink_def
+        pair_union_arcs_disj perm_face perm_on.cycle_count_skip perm_on.intro
+        pre_hypermap.select_convs(1) walkupE_def walkup_face z_dart)
+  ultimately have rhs_h': "euler_rhs H' = euler_rhs H + 1"
+    by (simp add: euler_rhs_def)
+  then consider (disconnected) "disconnected" | (connected) "\<not> disconnected" by auto
   then show ?thesis
-    sorry
+  proof cases
+    case disconnected
+    then have "card (pre_digraph.sccs (glink H')) = card (pre_digraph.sccs (glink H)) + 1"
+      by (metis False n_comp_glink_Walkup add.commute add.right_neutral n_comp_z_def)
+    then have "euler_lhs H' = euler_lhs H + 1"
+      by (metis False \<open>disconnected\<close> add.commute add.right_neutral
+          euler_lhs_walkupE mult_2_right n_comp_z_def)
+    then show ?thesis
+      by (simp add: genus_def rhs_h')
+  next
+    case connected
+    then have "card (pre_digraph.sccs (glink H')) = card (pre_digraph.sccs (glink H))"
+      by (metis False add.commute add_right_imp_eq n_comp_glink_Walkup n_comp_z_def)
+    then have "euler_lhs H' + 1 = euler_lhs H"
+      using euler_lhs_walkupE n_comp_glink_Walkup by auto
+    then show ?thesis
+      by (simp add: genus_def rhs_h')
+  qed
 qed
 
 lemma planar_walkupE: "planar H \<Longrightarrow> planar H'"
   by (metis bot.extremum_unique bot_nat_def le_genus_walkupE planar_def)
 
 lemma even_genus_walkupE: "even (genus H') \<Longrightarrow> even (genus H)"
-  sorry
-  (*by (smt (verit) euler_lhs_walkupE euler_rhs_walkupE genus_def)*)
+sorry
+
 
 lemma Jordan_WalkupE: "jordan \<Longrightarrow> hypermap.jordan H'"
-  sorry
+proof -
+  assume assm: "jordan"
+  obtain t where "node H t = z"
+      using nodeK by blast
+  then have "z\<rightarrow>\<^bsub>clink H\<^esub>t"
+    by (simp add: parcs_clink z_dart)
+  define clink1 where "clink1 \<equiv> pair_union (Gr (darts H') (skip_perm z (face H))) ((cnode H)\<^sup>R)"
+  then have clink1_verts: "verts clink1 = darts H"
+    by (metis (no_types, hide_lams) walkup_darts_subset pair_union_def  Gr_verts Un_iff cnode_def 
+        pair_pre_digraph.select_convs(1) reverse_def subset_antisym subset_iff with_proj_simps(1))
+  have cpath1I: "x \<noteq> z \<Longrightarrow> vwalk (x#p) (clink H') \<Longrightarrow> t \<notin> set p \<Longrightarrow> vwalk (x#p) clink1" for x p
+  proof (rule vwalkI; safe)
+    assume *: "x \<noteq> z" "vwalk (x # p) (clink H')" "t \<notin> set p"
+    show in_verts: "xa \<in> set (x # p) \<Longrightarrow> xa \<in> verts (with_proj clink1)" for xa
+      by (metis *(2) H'_def clink1_verts hypermap.hypermap_walkupE hypermap.verts_clink
+          hypermap_axioms subsetD vwalkE walkup_darts_subset with_proj_simps(1))
+    show "(a, b) \<in> set (vwalk_arcs (x # p)) \<Longrightarrow> a \<rightarrow>\<^bsub>clink1\<^esub> b" for a b
+    proof -
+      assume "(a, b) \<in> set (vwalk_arcs (x # p))"
+      have "a \<noteq> z \<and> b \<noteq> z"
+        by (metis "*"(2) DiffE H'_def \<open>(a, b) \<in> set (vwalk_arcs (x # p))\<close> hypermap.hypermap_walkupE 
+            hypermap.verts_clink hypermap_axioms in_set_vwalk_arcsE pre_hypermap.select_convs(1)
+            singletonI vwalk_verts_in_verts walkupE_def)
+      have "b \<noteq> t"
+        by (smt (verit, best) *(3) Pair_inject \<open>(a, b) \<in> set (vwalk_arcs (x # p))\<close> 
+            in_set_vwalk_arcsE list.distinct(1) list.inject list.set_cases list.set_intros(1)
+            vwalk_arcs.elims)
+      have "face H' a = b \<or> node H' b = a"
+        by (metis (no_types, lifting) "*"(2) H'_def \<open>(a, b) \<in> set (vwalk_arcs (x # p))\<close> 
+            hypermap.arc_clink hypermap.hypermap_walkupE hypermap.verts_clink hypermap_axioms 
+            in_set_vwalk_arcsE subsetD vwalkE)
+      moreover have "face H' a = b \<Longrightarrow> (a,b) \<in> parcs clink1"
+        by (metis (no_types, lifting) *(2) Gr_eq H'_def \<open>(a, b) \<in> set (vwalk_arcs (x # p))\<close>
+            arc_in_union clink1_def hypermap.hypermap_walkupE hypermap.verts_clink hypermap_axioms
+            in_mono in_set_vwalk_arcsE vwalkE walkup_face with_proj_simps(3))
+      moreover have "node H' b = a \<Longrightarrow> node H b = a"
+        by (metis \<open>(node H) \<langle>$\<rangle> t = z\<close> \<open>a \<noteq> z \<and> b \<noteq> z\<close> \<open>b \<noteq> t\<close> faceK skip_perm_invariant walkup_node)
+      ultimately show ?thesis
+        by (smt (z3) "*"(2) Gr_eq H'_def \<open>(a, b) \<in> set (vwalk_arcs (x # p))\<close> \<open>a \<noteq> z \<and> b \<noteq> z\<close>
+            arc_clink arc_reverse cface_def clink1_def clinkP hypermap.hypermap_walkupE 
+            hypermap.verts_clink hypermap_axioms in_mono in_set_vwalk_arcsE pair_union_arcs_disj 
+            skip_perm_invariant vwalkE walkup_darts_subset with_proj_simps(3))
+    qed
+  qed    
+  have cpathI: "x \<noteq> z \<Longrightarrow> vwalk (x#p) clink1 \<Longrightarrow> face H z \<notin> set p \<Longrightarrow> vwalk (x#p) (clink H)" for x p
+  proof (rule vwalkI; safe)
+    assume *: "x \<noteq> z" "vwalk (x # p) clink1" "face H z \<notin> set p"
+    show in_verts: "xa \<in> set (x # p) \<Longrightarrow> xa \<in> verts (clink H)" for xa
+      by (metis *(2) clink1_verts hypermap.verts_clink 
+          hypermap_axioms subsetD vwalkE with_proj_simps(1))
+    show "(a, b) \<in> set (vwalk_arcs (x # p)) \<Longrightarrow> a \<rightarrow>\<^bsub>clink H\<^esub> b" for a b
+    proof -
+      assume arc: "(a, b) \<in> set (vwalk_arcs (x # p))"
+      have "b \<noteq> face H z"
+        by (smt (verit, best) *(3) Pair_inject \<open>(a, b) \<in> set (vwalk_arcs (x # p))\<close> 
+            in_set_vwalk_arcsE list.distinct(1) list.inject list.set_cases list.set_intros(1)
+            vwalk_arcs.elims)
+      have "a\<rightarrow>\<^bsub>(Gr (darts H') (skip_perm z (face H)))\<^esub>b \<or> a\<rightarrow>\<^bsub>(cnode H)\<^sup>R\<^esub>b"
+        by (metis (no_types, lifting) arc *(2) clink1_def in_mono pair_union_arcs_disj vwalkE)
+      moreover have "a\<rightarrow>\<^bsub>(cnode H)\<^sup>R\<^esub>b \<Longrightarrow> (a,b) \<in> parcs (clink H)"
+        by (metis clink_def pair_union_arcs_disj with_proj_simps(3))
+      moreover have "a\<rightarrow>\<^bsub>(Gr (darts H') (skip_perm z (face H)))\<^esub>b \<Longrightarrow> (a,b) \<in> parcs (clink H)"
+        by (metis DiffE Gr_eq H'_def \<open>b \<noteq> (face H) \<langle>$\<rangle> z\<close> apply_skip_perm hypermap.arc_clink 
+            hypermap_axioms pre_hypermap.select_convs(1) singletonI skip_fz skip_perm_invariant
+            walkupE_def with_proj_simps(3))
+      ultimately show ?thesis
+        using with_proj_simps(3) by blast
+    qed
+  qed    
+  have cpath1P: "x \<noteq> z \<Longrightarrow> vwalk (x#p) clink1 \<Longrightarrow> \<not> vwalk (x#p) (clink H) \<Longrightarrow> distinct p \<Longrightarrow>
+              \<exists> p1 p2. face H z \<in> set p \<and> p = p1 @ p2 \<and> last (z#p2) = last (x#p) \<and> 
+    vwalk (x#p1@[z]) (clink H) \<and> vwalk (z#p2) (clink H)" for p x
+    sorry
+  {
+    assume *: "\<not> hypermap.jordan H'"
+    then obtain p where p_def: "hypermap.moebius_path H' p"
+      using H'_def hypermap.jordan_def hypermap_walkupE by auto
+    then obtain x q where "p = x#q"
+      by (metis H'_def hypermap.moebius_path.simps(1) hypermap_walkupE neq_Nil_conv)
+    then obtain y where "node H' y = last p"
+      by (meson eq_apply_perm_inverse_iff)
+    from this p_def have moebius_p: "appears_before q y (node H' x)" "vpath p (clink H')"
+      apply (smt (z3) \<open>p = x # q\<close> H'_def hypermap.faceK last_ConsR
+         hypermap.moebius_path.elims(1) hypermap.moebius_path.simps(2) hypermap_walkupE list.inject)
+      using H'_def hypermap.moebius_path.elims(2) hypermap_walkupE p_def by auto
+    then have Lp: "last p = (if y = t then node H z else node H y)"
+      by (metis DiffE H'_def \<open>(node H') \<langle>$\<rangle> y = last p\<close> \<open>(node H) \<langle>$\<rangle> t = z\<close> apply_inj_eq_iff 
+          apply_skip_perm hypermap.verts_clink hypermap_walkupE in_mono last_in_set 
+          pre_hypermap.select_convs(1) singletonI skip_fz skip_id skip_perm_invariant vpathE 
+          vwalkE walkupE_def walkup_node)
+    have pynx: "appears_before q y (if x = t then node H z else node H x)"
+      by (smt (z3) H'_def \<open>(node H) \<langle>$\<rangle> t = z\<close> \<open>p = x # q\<close> appears_before_in(2) apply_inj_eq_iff
+          apply_skip_perm distinct.simps(2) hypermap.moebius_path.elims(2) hypermap_walkupE
+          moebius_p(1) p_def skip_fz skip_id skip_perm_invariant vpathE walkup_node)
+    have "z \<notin> set p"
+      by (metis Diff_insert_absorb H'_def hypermap.hypermap_walkupE hypermap.verts_clink
+          hypermap_axioms mk_disjoint_insert moebius_p(2) pre_hypermap.select_convs(1) vpathE 
+          vwalk_verts_in_verts walkupE_def z_dart)
+    then have "distinct (z#p)"
+      using moebius_p(2) by auto
+    have "x \<noteq> y"
+      by (metis \<open>p = x # q\<close> appears_before_in(1) distinct.simps(2) moebius_p vpathE)
+    have "\<not> vwalk p (clink H)"
+    proof
+      assume "vwalk p (clink H)"
+      then have "vpath p (clink H)"
+        using moebius_p by blast
+      consider (x) "x = t \<and> y \<noteq> t" | (y) "x \<noteq> t \<and> y = t" | (neither) "x \<noteq> t \<and> y \<noteq> t"
+        using \<open>x \<noteq> y\<close> by auto
+      then have "\<exists>p. moebius_path p"
+      proof cases
+        case x
+        then have "appears_before q y (node H z)"
+          using pynx by auto
+        also have "vpath (z#p) (clink H)"
+          by (metis \<open>distinct (z # p)\<close> \<open>p = x # q\<close> \<open>vwalk p (clink H)\<close> \<open>z \<rightarrow>\<^bsub>with_proj (clink H)\<^esub> t\<close>
+              vpathI wf_clink wf_digraph.vwalk_Cons_Cons wf_digraph_wp_iff x)
+        ultimately have "moebius_path (z#p)"
+          by (metis Lp \<open>p = x # q\<close> appears_before_cons faceK moebius_path.simps(3) x)
+        then show ?thesis by blast
+      next
+        case y
+        then have "last p = node H z"
+          by (meson Lp)
+        then have "vpath (p@[z]) (clink H)"
+          using \<open>vpath p (clink H)\<close> \<open>z \<notin> set p\<close> clinkN disjoint_insert(1) 
+            distinct_append distinct_singleton insert_subset list.simps(15) set_vwalk_arcs_snoc
+            verts_clink vpath_def vwalk_def walkup.z_dart walkup_axioms by fastforce
+        also have "appears_before q y (node H x)"
+          using pynx y by auto
+        then have "appears_before (q@[z]) y (node H x)"
+          by (simp add: appears_before_append)
+        ultimately have "moebius_path (p@[z])"
+          by (smt (verit, del_insts) \<open>(node H) \<langle>$\<rangle> t = z\<close> \<open>p = x # q\<close> append_Cons 
+              append_is_Nil_conv hypermap.faceK hypermap.moebius_path.elims(1) hypermap_axioms
+              last_snoc list.distinct(1) list.inject y)
+        then show ?thesis by auto
+      next
+        case neither
+        then have "moebius_path p"
+          by (smt (z3) H'_def Lp \<open>p = x # q\<close> \<open>vpath p (clink H)\<close> \<open>vwalk p (clink H)\<close> hypermap.faceK
+              hypermap.moebius_path.elims(1) hypermap.moebius_path.simps(2) hypermap_axioms
+              hypermap_walkupE last_ConsR list.inject p_def pynx vwalk_def)
+        then show ?thesis by auto
+      qed
+      then show False
+        using assm jordan_def by auto
+    qed
+
+    have "\<not>vwalk p clink1"
+      sorry
+
+    then have "t \<in> set p"
+      using \<open>distinct (z # p)\<close> \<open>p = x # q\<close> cpath1I moebius_p(2) by auto
+
+    then have "appears_before q y (node H x)"
+      by (metis (mono_tags, hide_lams) \<open>\<not> vwalk p (with_proj clink1)\<close> \<open>p = x # q\<close> 
+          cpath1I distinct.simps(2) moebius_p(2) pynx vpathE)
+
+    obtain p1 p2 where p12_def: "p1 @ (t#p2) = q"
+      by (metis \<open>\<not> vwalk p clink1\<close> \<open>distinct (z # p)\<close> \<open>p = x # q\<close> cpath1I 
+          distinct_length_2_or_more moebius_p(2) split_list vpathE)
+    then have "set p1 \<inter> set p2 = {}"
+      using \<open>distinct (z # p)\<close> \<open>p = x # q\<close> by force
+    have "vpath (t#p2) clink1"
+      by (metis \<open>p = x # q\<close> \<open>t \<in> set p\<close> \<open>z \<notin> set p\<close> append_is_Nil_conv cpath1I distinct.simps(2)
+        distinct_append list.distinct(1) moebius_p(2) vpath_def vwalkI_append_r vwalk_consE p12_def)
+    have "vpath (x#p1) clink1"
+      unfolding vpath_def apply auto
+        apply (rule cpath1I)
+          using \<open>p = x # q\<close> \<open>z \<notin> set p\<close> apply force
+          apply (metis \<open>p = x # q\<close> p12_def moebius_p(2) append_Cons
+                       list.discI vpath_def vwalkI_append_l)
+          using \<open>distinct (z # p)\<close> \<open>p = x # q\<close> \<open>p1 @ t # p2 = q\<close> apply fastforce+
+    done
+    have Lp1: "last (x#p1) = node H z"
+      sorry
+    have Lp2: "last (t#p2) = node H y \<and> y \<noteq> t"
+      by (metis Lp Lp1 \<open>p = x # q\<close> append_is_Nil_conv disjoint_insert(1) distinct.simps(2) 
+          distinct_append insert_Diff last.simps last_appendR last_in_set list.distinct(1) 
+          moebius_p(2) p12_def vpathE)
+    have xCp1: "vpath (x#p1) (clink H)"
+      sorry
+
+    have "\<not> vpath (t#p2) (clink H)"
+    proof
+      assume "vpath (t # p2) (clink H)"
+      then have "vpath (z#t#p2) (clink H)"
+        by (metis Un_iff \<open>distinct (z # p)\<close> \<open>p = x # q\<close> \<open>z \<rightarrow>\<^bsub>with_proj (clink H)\<^esub> t\<close>
+            distinct.simps(2) distinct_length_2_or_more fin_digraph.axioms(1) finite_clink p12_def 
+            set_append vpath_def wf_digraph.vwalk_Cons_Cons)
+      also have "vwalk (x#p1@[z]) (clink H)"
+        by (smt (verit, ccfv_threshold) Lp1 xCp1 Un_insert_right append_Cons append_Nil2 clinkN 
+            insert_subset list.distinct(1) list.simps(15) set_append set_vwalk_arcs_snoc
+            verts_clink vpathE vwalk_def walkup.z_dart walkup_axioms)
+      ultimately have "vpath (x#p1@(z#t#p2)) (clink H)"
+        sorry
+      then have "moebius_path (x#p1@(z#t#p2))"
+        sorry
+      then show False
+        using assm jordan_def by blast
+    qed
+    obtain q1 q2 where "p2 = q1 @ q2"
+      by blast
+
+    have "y \<notin> set (t # q1)"
+      sorry
+
+    have "node H x \<in> set (t # q1)"
+      sorry
+
+    have "y \<in> set p1"
+      sorry
+
+    then have False
+      sorry
+  }
+    then show ?thesis
+      by blast
+qed
+
 end
 
 section \<open>Other walkups\<close>
+
 
 definition "walkupN H z \<equiv> permF (walkupE (permN H) z)"
 
 definition "walkupF H z \<equiv> permN (walkupE (permF H) z)"
 
-lemma (in walkup) planar_walkupN: "planar H \<Longrightarrow> planar (walkupN H z)"
+definition skip_node where
+"skip_node z h x \<equiv> if z = x then z else
+                  (if (node h z) = z then node h x else
+                  (if x = face h z then node h z else
+                  (if node h x = z then node h (face h z) else node h x)))"
+
+definition skip_face where
+"skip_face z h x \<equiv> if z = x then z else
+                  (if (face h z) = z then face h x else
+                  (if x = edge h z then face h z else
+                  (if face h x = z then face h (edge h z) else face h x)))"
+
+context walkup begin
+
+lemma darts_walkupN: "darts (walkupN H z) = darts H - {z}"
+  by (simp add: permF_def permN_def walkupE_def walkupN_def)
+
+lemma darts_walkupF: "darts (walkupF H z) = darts H - {z}"
+  by (simp add: permF_def permN_def walkupE_def walkupF_def)
+
+lemma card_walkupN: "card (darts (walkupN H z)) = card (darts H) - 1"
+  by (simp add: darts_walkupN finite_darts z_dart)
+
+lemma card_walkupF: "card (darts (walkupF H z)) = card (darts H) - 1"
+  by (simp add: darts_walkupF finite_darts z_dart)
+
+lemma edge_walkupN: "edge (walkupN H z) = skip_perm z (edge H)"
+  by (simp add: permF_def permN_def walkupE_def walkupN_def)
+
+lemma node_walkupN: "node (walkupN H z) x = skip_node z H x"
+  by (smt (z3) hypermap.skip_edge_Perm hypermap_permN permF_def permN_def 
+      pre_hypermap.select_convs(2) pre_hypermap.select_convs(3) skip_edge_def 
+      skip_node_def walkupE_def walkupN_def)
+
+lemma face_walkupN: "face (walkupN H z) = skip_perm z (face H)"
+  by (simp add: permF_def permN_def walkupE_def walkupN_def)
+
+lemma edge_walkupF: "edge (walkupF H z) = skip_perm z (edge H)"
+  by (simp add: permF_def permN_def walkupE_def walkupF_def)
+
+lemma node_walkupF: "node (walkupF H z) = skip_perm z (node H)"
+  by (simp add: permF_def permN_def walkupE_def walkupF_def)
+
+lemma face_walkupF: "face (walkupF H z) x = skip_face z H x"
+  by (smt (z3) hypermap.skip_edge_Perm hypermap_permF permF_def permN_def 
+      pre_hypermap.select_convs(2) pre_hypermap.select_convs(3) pre_hypermap.select_convs(4)
+      skip_edge_def skip_face_def walkupE_def walkupF_def)
+
+lemma planar_walkupN: "planar H \<Longrightarrow> planar (walkupN H z)"
 proof -
   assume *: "planar H"
   then have "planar (walkupE (permN H) z)"
     by (metis hypermap_permN permN_def planar_permN pre_hypermap.select_convs(1) walkup.H'_def
         walkup.planar_walkupE walkup_axioms.intro walkup_def z_dart)
   then show ?thesis
-    by (metis hypermap.genus_permF hypermap_permN permN_def planar_def pre_hypermap.select_convs(1)
-        walkup.H'_def walkup.hypermap_walkupE walkup.intro walkupN_def walkup_axioms.intro z_dart)
+    by (simp add: hypermap.genus_permF hypermap.hypermap_walkupE hypermap_permN planar_def walkupN_def)
 qed
 
-lemma (in walkup) planar_walkupF: "planar H \<Longrightarrow> planar (walkupF H z)"
+lemma planar_walkupF: "planar H \<Longrightarrow> planar (walkupF H z)"
 proof -
   assume *: "planar H"
   then have "planar (walkupE (permF H) z)"
     by (metis hypermap_permF permF_def planar_permF pre_hypermap.select_convs(1) walkup.H'_def
         walkup.planar_walkupE walkup_axioms.intro walkup_def z_dart)
   then show ?thesis
-    by (metis hypermap.genus_permN hypermap_permF permF_def planar_def pre_hypermap.select_convs(1)
-        walkup.H'_def walkup.hypermap_walkupE walkup.intro walkupF_def walkup_axioms.intro z_dart)
+    by (simp add: hypermap.genus_permN hypermap.hypermap_walkupE
+        hypermap_permF planar_def walkupF_def)
 qed
+
+end
 
 end
